more beta

Church.v
@@ -6,9 +6,6 @@ Fixpoint _mk_app (n: nat) :=
   | S n => app (var 1) (_mk_app n)
  end.
 
-Definition nat_to_church (n: nat): LambdaTerm :=
-  abst (abst (_mk_app n)).
-
 Fixpoint _app_to_nat (t: LambdaTerm): (option nat) :=
   match t with
     | var 0 => Some 0
@@ -22,11 +19,30 @@ Fixpoint _app_to_nat (t: LambdaTerm): (option nat) :=
 Definition church_succ := 
   (abst (abst (abst (app (var 1) (app (app (var 2) (var 1)) (var 0)))))).
 
+Definition church_true := (abst (abst (var 1))).
+Definition church_false := (abst (abst (var 0))).
+Definition church_and := (abst (abst (app (app (var 1) (var 0)) (var 1)))).
+Definition church_or := (abst (abst (app (app (var 1) (var 1)) (var 0)))).
+Definition church_not := (abst (abst (abst (app (app (var 2) (var 0)) (var 1))))).
+Definition church_xor := (abst (abst (app (app (var 1) (app church_not (var 0))) (var 0)))).
+Definition church_if := (abst (abst (abst (app (app (var 2) (var 1)) (var 0))))).
+Definition church_pair := (abst (abst (abst (app (app (var 0) (var 2)) (var 1))))).
+Definition church_first := (abst (app (var 0) (abst (abst (var 1))))).
+Definition church_second := (abst (app (var 0) (abst (abst (var 0))))).
+Definition church_is_zero := (abst (app (app (var 0) (abst church_false)) church_true)).
+Definition bool_to_church (b: bool): LambdaTerm :=
+match b with
+| true => church_true
+| false => church_false
+end.
+
+Definition church_to_bool (ch: LambdaTerm): bool := lambda_eq ch church_true.
+
+Definition nat_to_church (n: nat): LambdaTerm :=
+  abst (abst (_mk_app n)).
+
 Definition church_to_nat (ch: LambdaTerm): (option nat) :=
   match ch with
     | (abst (abst a)) => _app_to_nat a
     | _ => None
   end.
-
-Definition church_true := (abst (abst (var 1))).
-Definition church_false := (abst (abst (var 0))).
