Beta.v
@@ -14,6 +14,7 @@ end.
 (* depth = 0 -> 'every variable is free' *)
 (* depth = 1 -> 'every variable except 0 is free' *)
 (* depth = 2 -> 'every variable except 0, 1 is free' *)
+(* depth = n -> 'every variable < n is free' *)
 Fixpoint inc_free_vars (t: LambdaTerm) (depth: nat) (amount: nat): LambdaTerm :=
 match t with
 | var n => if (depth <=? n)
@@ -44,6 +45,8 @@ match t with
 | _ => t
 end.
 
+Definition RBeta (a b: LambdaTerm): Prop := (beta a) = b.
+
 Fixpoint _beta_fuel (t: LambdaTerm) (fuel: nat): LambdaTerm :=
   match fuel with
   | 0 => t
@@ -55,3 +58,12 @@ Fixpoint _beta_fuel (t: LambdaTerm) (fuel: nat): LambdaTerm :=
 
 Definition beta_fuel (t: LambdaTerm): LambdaTerm :=
   _beta_fuel t 100.
+
+Definition betan (t: LambdaTerm): LambdaTerm :=
+  beta (beta t).
+
+Definition beta3 (t: LambdaTerm): LambdaTerm :=
+  beta (beta (beta t)).
+
+Definition beta4 (t: LambdaTerm): LambdaTerm :=
+  beta (beta (beta (beta t))).
