ChurchTests.v
@@ -1,0 +1,73 @@
+Require Import LambdaDebrujin.
+Require Import Beta.
+Require Import Church.
+
+Example succ_test_0:
+ (beta_fuel (app church_succ (nat_to_church 0))) = (nat_to_church 1).
+Proof. simpl. reflexivity. Qed.
+
+Example succ_test_1:
+ (beta_fuel (app church_succ (nat_to_church 1))) = (nat_to_church 2).
+Proof. simpl. reflexivity. Qed.
+
+Example succ_test_2:
+ (beta_fuel (app church_succ (nat_to_church 2))) = (nat_to_church 3).
+Proof. simpl. reflexivity. Qed.
+
+Example and_check:
+ forall a b: bool, (beta_fuel (app (app church_and (bool_to_church a)) (bool_to_church b))) = bool_to_church (andb a b).
+Proof. 
+ destruct a, b.
+ - simpl. reflexivity. 
+ - simpl. reflexivity. 
+ - simpl. reflexivity. 
+ - simpl. reflexivity. 
+Qed.
+
+Example or_check:
+ forall a b: bool, (beta_fuel (app (app church_or (bool_to_church a)) (bool_to_church b))) = bool_to_church (orb a b).
+Proof. 
+ destruct a, b.
+ - simpl. reflexivity. 
+ - simpl. reflexivity. 
+ - simpl. reflexivity. 
+ - simpl. reflexivity. 
+Qed.
+
+Example xor_check:
+ forall a b: bool, (beta_fuel (app (app church_xor (bool_to_church a)) (bool_to_church b))) = bool_to_church (xorb a b).
+Proof. 
+ destruct a, b.
+ - simpl. reflexivity.
+ - simpl. reflexivity.
+ - simpl. reflexivity.
+ - simpl. reflexivity.
+Qed.
+
+Example not_check:
+ forall a: bool, beta_fuel (app church_not (bool_to_church a)) = bool_to_church (negb a).
+Proof. 
+ destruct a.
+ - simpl. reflexivity.
+ - simpl. reflexivity.
+Qed.
+
+Example test_if_true:
+ beta_fuel (app (app (app church_if church_true) (nat_to_church 42)) (nat_to_church 17)) = (nat_to_church 42).
+Proof. simpl. reflexivity. Qed.
+
+Example test_if_false:
+ beta_fuel (app (app (app church_if church_false) (nat_to_church 42)) (nat_to_church 17)) = (nat_to_church 17).
+Proof. simpl. reflexivity. Qed.
+
+Example test_if_zero:
+ beta_fuel (app church_is_zero (nat_to_church 0)) = church_true.
+Proof. simpl. reflexivity. Qed.
+
+Example test_pair_first: 
+ beta_fuel (app church_first (app (app church_pair (nat_to_church 2)) (nat_to_church 3))) = nat_to_church 2.
+Proof. simpl. reflexivity. Qed.
+
+Example test_pair_second: 
+ beta_fuel (app church_second (app (app church_pair (nat_to_church 2)) (nat_to_church 3))) = nat_to_church 3.
+Proof. simpl. reflexivity. Qed.
