LambdaInLambda.v
@@ -1,0 +1,16 @@
+Require Import LambdaDebrujin.
+Require Import Church.
+Require Import Beta.
+
+Fixpoint encode_lambda (t: LambdaTerm) := 
+let zero := nat_to_church 0 in
+let one := nat_to_church 1 in
+let two := nat_to_church 2 in
+match t with
+| var n => app (app church_pair zero) (nat_to_church n)
+| app a b => app (app church_pair one) 
+                 (app (app church_pair (encode_lambda a)) 
+                      (app church_pair (encode_lambda b)))
+| abst body => app (app church_pair two) (encode_lambda body)
+end.
+
